spec/abstract/Schedule_A.thy
@@ -15,7 +15,7 @@ Non-deterministic scheduler functionality.
 chapter "Scheduler"
 
 theory Schedule_A
-imports Arch_A
+imports "./$L4V_ARCH/Arch_A"
 begin
 
 abbreviation
