spec/design/ARM/ArchInterruptDecls_H.thy
@@ -1,0 +1,22 @@
+(*
+ * Copyright 2014, General Dynamics C4 Systems
+ *
+ * This software may be distributed and modified according to the terms of
+ * the GNU General Public License version 2. Note that NO WARRANTY is provided.
+ * See "LICENSE_GPLv2.txt" for details.
+ *
+ * @TAG(GD_GPL)
+ *)
+
+theory ArchInterruptDecls_H
+imports "../RetypeDecls_H" "../CNode_H" 
+begin
+
+consts
+decodeIRQControl :: "machine_word \<Rightarrow> machine_word list \<Rightarrow> machine_word \<Rightarrow> capability list \<Rightarrow> ( syscall_error , ArchRetypeDecls_H.irqcontrol_invocation ) kernel_f"
+
+consts
+performIRQControl :: "ArchRetypeDecls_H.irqcontrol_invocation \<Rightarrow> unit kernel_p"
+
+
+end
