spec/design/ARM/ArchInterrupt_H.thy
@@ -1,0 +1,22 @@
+(*
+ * Copyright 2014, General Dynamics C4 Systems
+ *
+ * This software may be distributed and modified according to the terms of
+ * the GNU General Public License version 2. Note that NO WARRANTY is provided.
+ * See "LICENSE_GPLv2.txt" for details.
+ *
+ * @TAG(GD_GPL)
+ *)
+
+theory ArchInterrupt_H
+imports "../RetypeDecls_H" "../CNode_H" "../InterruptDecls_H" ArchInterruptDecls_H
+begin
+
+defs decodeIRQControl_def:
+"decodeIRQControl arg1 arg2 arg3 arg4 \<equiv> throw IllegalOperation"
+
+defs performIRQControl_def:
+"performIRQControl arg1 \<equiv> haskell_fail []"
+
+
+end
