spec/design/ARM/ArchInvocationLabels_H.thy
@@ -1,0 +1,94 @@
+(*
+ * Copyright 2014, General Dynamics C4 Systems
+ *
+ * This software may be distributed and modified according to the terms of
+ * the GNU General Public License version 2. Note that NO WARRANTY is provided.
+ * See "LICENSE_GPLv2.txt" for details.
+ *
+ * @TAG(GD_GPL)
+ *)
+
+chapter "Architecture-specific Invocation Labels"
+
+theory ArchInvocationLabels_H
+imports "../../../lib/Enumeration"
+begin
+
+text {*
+  An enumeration of arch-specific system call labels.
+*}
+
+datatype arch_invocation_label =
+    ARMPDClean_Data
+  | ARMPDInvalidate_Data
+  | ARMPDCleanInvalidate_Data
+  | ARMPDUnify_Instruction
+  | ARMPageTableMap
+  | ARMPageTableUnmap
+  | ARMPageMap
+  | ARMPageRemap
+  | ARMPageUnmap
+  | ARMPageClean_Data
+  | ARMPageInvalidate_Data
+  | ARMPageCleanInvalidate_Data
+  | ARMPageUnify_Instruction
+  | ARMPageGetAddress
+  | ARMASIDControlMakePool
+  | ARMASIDPoolAssign
+
+(* arch_invocation_label instance proofs *)
+(*<*)
+instantiation arch_invocation_label :: enum begin
+definition
+  enum_arch_invocation_label: "enum_class.enum \<equiv> 
+    [ 
+      ARMPDClean_Data,
+      ARMPDInvalidate_Data,
+      ARMPDCleanInvalidate_Data,
+      ARMPDUnify_Instruction,
+      ARMPageTableMap,
+      ARMPageTableUnmap,
+      ARMPageMap,
+      ARMPageRemap,
+      ARMPageUnmap,
+      ARMPageClean_Data,
+      ARMPageInvalidate_Data,
+      ARMPageCleanInvalidate_Data,
+      ARMPageUnify_Instruction,
+      ARMPageGetAddress,
+      ARMASIDControlMakePool,
+      ARMASIDPoolAssign
+    ]"
+
+
+definition
+  "enum_class.enum_all (P :: arch_invocation_label \<Rightarrow> bool) \<longleftrightarrow> Ball UNIV P"
+
+definition
+  "enum_class.enum_ex (P :: arch_invocation_label \<Rightarrow> bool) \<longleftrightarrow> Bex UNIV P"
+
+  instance
+  apply intro_classes
+   apply (safe, simp)
+   apply (case_tac x)
+  apply (simp_all add: enum_arch_invocation_label enum_all_arch_invocation_label_def enum_ex_arch_invocation_label_def)
+  by fast+
+end
+
+instantiation arch_invocation_label :: enum_alt
+begin
+definition
+  enum_alt_arch_invocation_label: "enum_alt \<equiv> 
+    alt_from_ord (enum :: arch_invocation_label list)"
+instance ..
+end
+
+instantiation arch_invocation_label :: enumeration_both
+begin
+instance by (intro_classes, simp add: enum_alt_arch_invocation_label)
+end
+
+(*>*)
+
+
+end
