spec/design/ARM/ArchRetype_H.thy
@@ -1,0 +1,297 @@
+(*
+ * Copyright 2014, General Dynamics C4 Systems
+ *
+ * This software may be distributed and modified according to the terms of
+ * the GNU General Public License version 2. Note that NO WARRANTY is provided.
+ * See "LICENSE_GPLv2.txt" for details.
+ *
+ * @TAG(GD_GPL)
+ *)
+
+chapter "Retyping Objects"
+
+theory ArchRetype_H
+imports
+  ArchRetypeDecls_H
+  ArchVSpaceDecls_H
+  Hardware_H
+  "../KI_Decls_H"
+begin
+
+defs deriveCap_def:
+"deriveCap x0 x1\<equiv> (let c = x1 in
+  if isPageTableCap c \<and> capPTMappedAddress c \<noteq> None
+  then   returnOk c
+  else if isPageTableCap c \<and> capPTMappedAddress c = None
+  then   throw IllegalOperation
+  else if isPageDirectoryCap c \<and> capPDMappedASID c \<noteq> None
+  then   returnOk c
+  else if isPageDirectoryCap c \<and> capPDMappedASID c = None
+  then   throw IllegalOperation
+  else if isPageCap c
+  then   returnOk $ c \<lparr> capVPMappedAddress := Nothing \<rparr>
+  else if isASIDControlCap c
+  then   returnOk c
+  else if isASIDPoolCap c
+  then   returnOk c
+  else undefined
+  )"
+
+defs updateCapData_def:
+"updateCapData arg1 arg2 cap \<equiv> ArchObjectCap cap"
+
+defs maskCapRights_def:
+"maskCapRights r x1\<equiv> (let c = x1 in
+  if isPageCap c
+  then   ArchObjectCap $ c \<lparr>
+    capVPRights := maskVMRights (capVPRights c) r \<rparr>
+  else   ArchObjectCap c
+  )"
+
+defs finaliseCap_def:
+"finaliseCap x0 x1\<equiv> (case (x0, x1) of
+    ((ASIDPoolCap ptr b), True) \<Rightarrow>    (do
+    deleteASIDPool b ptr;
+    return NullCap
+    od)
+  | ((PageDirectoryCap ptr (Some a)), True) \<Rightarrow>    (do
+    deleteASID a ptr;
+    return NullCap
+  od)
+  | ((PageTableCap ptr (Some (a, v))), True) \<Rightarrow>    (do
+    unmapPageTable a v ptr;
+    return NullCap
+  od)
+  | ((PageCap ptr _ s (Some (a, v))), _) \<Rightarrow>    (do
+        unmapPage s a v ptr;
+        return NullCap
+  od)
+  | (_, _) \<Rightarrow>    return NullCap
+  )"
+
+defs resetMemMapping_def:
+"resetMemMapping x0\<equiv> (case x0 of
+    (PageCap p rts sz _) \<Rightarrow>    PageCap p rts sz Nothing
+  | (PageTableCap ptr _) \<Rightarrow>    PageTableCap ptr Nothing
+  | (PageDirectoryCap ptr _) \<Rightarrow>    PageDirectoryCap ptr Nothing
+  | cap \<Rightarrow>    cap
+  )"
+
+defs recycleCap_def:
+"recycleCap is_final x1 \<equiv> (let cap = x1 in
+  if isPageCap cap
+  then   (do
+      doMachineOp $ clearMemory (capVPBasePtr cap)
+          (1 `~shiftL~` (pageBitsForSize $ capVPSize cap));
+      finaliseCap cap is_final;
+      return $ resetMemMapping cap
+  od)
+  else if isPageTableCap cap
+  then let ptr = capPTBasePtr cap
+  in   (do
+    pteBits \<leftarrow> return ( objBits InvalidPTE);
+    slots \<leftarrow> return ( [ptr, ptr + bit pteBits  .e.  ptr + bit ptBits - 1]);
+    mapM_x (flip storePTE InvalidPTE) slots;
+    doMachineOp $
+        cleanCacheRange_PoU (VPtr $ fromPPtr ptr)
+                            (VPtr $ fromPPtr ptr + (1 `~shiftL~` ptBits) - 1)
+                            (addrFromPPtr ptr);
+    (case capPTMappedAddress cap of
+          None \<Rightarrow>   return ()
+        | Some (a, v) \<Rightarrow>   (do
+            mapped \<leftarrow> pageTableMapped a v ptr;
+            when (mapped \<noteq> Nothing) $ invalidateTLBByASID a
+        od)
+        );
+    finaliseCap cap is_final;
+    return (if is_final then resetMemMapping cap else cap)
+  od)
+  else if isPageDirectoryCap cap
+  then let ptr = capPDBasePtr cap
+  in   (do
+    pdeBits \<leftarrow> return ( objBits InvalidPDE);
+    kBaseEntry \<leftarrow> return ( fromVPtr kernelBase
+                        `~shiftR~` pageBitsForSize ARMSection);
+    indices \<leftarrow> return ( [0  .e.  kBaseEntry - 1]);
+    offsets \<leftarrow> return ( map (PPtr \<circ> flip shiftL pdeBits) indices);
+    slots \<leftarrow> return ( map (\<lambda> x. x + ptr) offsets);
+    mapM_x (flip storePDE InvalidPDE) slots;
+    doMachineOp $
+        cleanCacheRange_PoU (VPtr $ fromPPtr ptr)
+                            (VPtr $ fromPPtr ptr + (1 `~shiftL~` pdBits) - 1)
+                            (addrFromPPtr ptr);
+    (case capPDMappedASID cap of
+          None \<Rightarrow>   return ()
+        | Some a \<Rightarrow>   (
+            ignoreFailure $ ((doE
+                pd' \<leftarrow> findPDForASID a;
+                withoutFailure $ when (ptr = pd') $ invalidateTLBByASID a
+            odE)
+                                                                          )
+        )
+        );
+    finaliseCap cap is_final;
+    return (if is_final then resetMemMapping cap else cap)
+  od)
+  else if isASIDControlCap cap
+  then   return ASIDControlCap
+  else if isASIDPoolCap cap
+  then let base = capASIDBase cap; ptr = capASIDPool cap
+  in   (do
+    asidTable \<leftarrow> gets (armKSASIDTable \<circ> ksArchState);
+    when (asidTable (asidHighBitsOf base) = Just ptr) $ (do
+        deleteASIDPool base ptr;
+        setObject ptr (makeObject ::asidpool);
+        asidTable \<leftarrow> gets (armKSASIDTable \<circ> ksArchState);
+        asidTable' \<leftarrow> return ( asidTable aLU [(asidHighBitsOf base, Just ptr)]);
+        modify (\<lambda> s. s \<lparr>
+            ksArchState := (ksArchState s) \<lparr> armKSASIDTable := asidTable' \<rparr>\<rparr>)
+    od);
+    return cap
+  od)
+  else undefined
+  )"
+
+defs hasRecycleRights_def:
+"hasRecycleRights x0\<equiv> (case x0 of
+    (PageCap _ rights _ _) \<Rightarrow>    rights = VMReadWrite
+  | _ \<Rightarrow>    True
+  )"
+
+defs sameRegionAs_def:
+"sameRegionAs x0 x1\<equiv> (let (a, b) = (x0, x1) in
+  if isPageCap a \<and> isPageCap b
+  then 
+    let
+        botA = capVPBasePtr a;
+        botB = capVPBasePtr b;
+        topA = botA + bit (pageBitsForSize $ capVPSize a) - 1;
+        topB = botB + bit (pageBitsForSize $ capVPSize b) - 1
+    in
+    
+    (botA \<le> botB) \<and> (topA \<ge> topB) \<and> (botB \<le> topB)
+  else if isPageTableCap a \<and> isPageTableCap b
+  then  
+    capPTBasePtr a = capPTBasePtr b
+  else if isPageDirectoryCap a \<and> isPageDirectoryCap b
+  then  
+    capPDBasePtr a = capPDBasePtr b
+  else if isASIDControlCap a \<and> isASIDControlCap b
+  then   True
+  else if isASIDPoolCap a \<and> isASIDPoolCap b
+  then  
+    capASIDPool a = capASIDPool b
+  else   False
+  )"
+
+defs isPhysicalCap_def:
+"isPhysicalCap x0\<equiv> (case x0 of
+    ASIDControlCap \<Rightarrow>    False
+  | _ \<Rightarrow>    True
+  )"
+
+defs sameObjectAs_def:
+"sameObjectAs x0 x1\<equiv> (let (a, b) = (x0, x1) in
+  if isPageCap a \<and> isPageCap b
+  then let ptrA = capVPBasePtr a
+  in  
+    (ptrA = capVPBasePtr b) \<and> (capVPSize a = capVPSize b)
+        \<and> (ptrA \<le> ptrA + bit (pageBitsForSize $ capVPSize a) - 1)
+  else   sameRegionAs a b
+  )"
+
+definition
+"createPageObject ptr numPages\<equiv> (do
+    addrs \<leftarrow> placeNewObject ptr UserData numPages;
+    doMachineOp $ initMemory (PPtr $ fromPPtr ptr) (1 `~shiftL~` (pageBits + numPages) );
+    return addrs
+od)"
+
+defs createObject_def:
+"createObject t regionBase arg3 \<equiv>
+    let funupd = (\<lambda> f x v y. if y = x then v else f y) in
+    let pointerCast = PPtr \<circ> fromPPtr
+    in (case t of 
+        ArchTypes_H.APIObjectType v1 \<Rightarrow> 
+            haskell_fail []
+        | ArchTypes_H.SmallPageObject \<Rightarrow>  (do
+            createPageObject regionBase 0;
+            modify (\<lambda> ks. ks \<lparr> gsUserPages :=
+              funupd (gsUserPages ks)
+                     (fromPPtr regionBase) (Just ARMSmallPage)\<rparr>);
+            return $ PageCap (pointerCast regionBase)
+                  VMReadWrite ARMSmallPage Nothing
+        od)
+        | ArchTypes_H.LargePageObject \<Rightarrow>  (do
+            createPageObject regionBase 4;
+            modify (\<lambda> ks. ks \<lparr> gsUserPages :=
+              funupd (gsUserPages ks)
+                     (fromPPtr regionBase) (Just ARMLargePage)\<rparr>);
+            return $ PageCap (pointerCast regionBase)
+                  VMReadWrite ARMLargePage Nothing
+        od)
+        | ArchTypes_H.SectionObject \<Rightarrow>  (do
+            createPageObject regionBase 8;
+            modify (\<lambda> ks. ks \<lparr> gsUserPages :=
+              funupd (gsUserPages ks)
+                     (fromPPtr regionBase) (Just ARMSection)\<rparr>);
+            return $ PageCap (pointerCast regionBase)
+                  VMReadWrite ARMSection Nothing
+        od)
+        | ArchTypes_H.SuperSectionObject \<Rightarrow>  (do
+            createPageObject regionBase 12;
+            modify (\<lambda> ks. ks \<lparr> gsUserPages :=
+              funupd (gsUserPages ks)
+                     (fromPPtr regionBase) (Just ARMSuperSection)\<rparr>);
+            return $ PageCap (pointerCast regionBase)
+                  VMReadWrite ARMSuperSection Nothing
+        od)
+        | ArchTypes_H.PageTableObject \<Rightarrow>  (do
+            ptSize \<leftarrow> return ( ptBits - objBits (makeObject ::pte));
+            regionSize \<leftarrow> return ( (1 `~shiftL~` ptBits));
+            placeNewObject regionBase (makeObject ::pte) ptSize;
+            doMachineOp $
+                cleanCacheRange_PoU (VPtr $ fromPPtr regionBase)
+                      (VPtr $ fromPPtr regionBase + regionSize - 1)
+                      (addrFromPPtr regionBase);
+            return $ PageTableCap (pointerCast regionBase) Nothing
+        od)
+        | ArchTypes_H.PageDirectoryObject \<Rightarrow>  (do
+            pdSize \<leftarrow> return ( pdBits - objBits (makeObject ::pde));
+            regionSize \<leftarrow> return ( (1 `~shiftL~` pdBits));
+            placeNewObject regionBase (makeObject ::pde) pdSize;
+            copyGlobalMappings (pointerCast regionBase);
+            doMachineOp $
+                cleanCacheRange_PoU (VPtr $ fromPPtr regionBase)
+                      (VPtr $ fromPPtr regionBase + regionSize - 1)
+                      (addrFromPPtr regionBase);
+            return $ PageDirectoryCap (pointerCast regionBase) Nothing
+        od)
+        )"
+
+defs decodeInvocation_def:
+"decodeInvocation \<equiv> decodeARMMMUInvocation"
+
+defs performInvocation_def:
+"performInvocation \<equiv> performARMMMUInvocation"
+
+defs capUntypedPtr_def:
+"capUntypedPtr x0\<equiv> (case x0 of
+    (PageCap ((* PPtr *) p) _ _ _) \<Rightarrow>    PPtr p
+  | (PageTableCap ((* PPtr *) p) _) \<Rightarrow>    PPtr p
+  | (PageDirectoryCap ((* PPtr *) p) _) \<Rightarrow>    PPtr p
+  | ASIDControlCap \<Rightarrow>    error []
+  | (ASIDPoolCap ((* PPtr *) p) _) \<Rightarrow>    PPtr p
+  )"
+
+defs capUntypedSize_def:
+"capUntypedSize x0\<equiv> (case x0 of
+    (PageCap _ _ sz _) \<Rightarrow>    1 `~shiftL~` pageBitsForSize sz
+  | (PageTableCap _ _) \<Rightarrow>    1 `~shiftL~` 10
+  | (PageDirectoryCap _ _) \<Rightarrow>    1 `~shiftL~` 14
+  | (ASIDControlCap ) \<Rightarrow>    1 `~shiftL~` (asidHighBits + 2)
+  | (ASIDPoolCap _ _) \<Rightarrow>    1 `~shiftL~` (asidLowBits + 2)
+  )"
+
+
+end
