spec/design/Interrupt_H.thy
@@ -11,54 +11,23 @@
 theory Interrupt_H
 imports
   RetypeDecls_H
-  ArchInterrupt_H
+  "./$L4V_ARCH/ArchInterrupt_H"
   Notification_H
   CNode_H
   KI_Decls_H
+  InterruptDecls_H
 begin
 
-consts
-decodeIRQControlInvocation :: "machine_word \<Rightarrow> machine_word list \<Rightarrow> machine_word \<Rightarrow> capability list \<Rightarrow> ( syscall_error , irqcontrol_invocation ) kernel_f"
-
-consts
-invokeIRQControl :: "irqcontrol_invocation \<Rightarrow> unit kernel_p"
-
-consts
-decodeIRQHandlerInvocation :: "machine_word \<Rightarrow> machine_word list \<Rightarrow> irq \<Rightarrow> (capability * machine_word) list \<Rightarrow> ( syscall_error , irqhandler_invocation ) kernel_f"
-
-consts
-toBool :: "machine_word \<Rightarrow> bool"
-
-consts
-invokeIRQHandler :: "irqhandler_invocation \<Rightarrow> unit kernel"
-
-consts
-deletingIRQHandler :: "irq \<Rightarrow> unit kernel"
-
-consts
-initInterruptController :: "capability \<Rightarrow> machine_word \<Rightarrow> capability kernel_init"
-
-consts
-handleInterrupt :: "irq \<Rightarrow> unit kernel"
-
-consts
-isIRQActive :: "irq \<Rightarrow> bool kernel"
-
-consts
-setIRQState :: "irqstate \<Rightarrow> irq \<Rightarrow> unit kernel"
-
-consts
-getIRQState :: "irq \<Rightarrow> irqstate kernel"
-
-consts
-getIRQSlot :: "irq \<Rightarrow> (machine_word) kernel"
+abbreviation (input)
+  performIRQControl :: "Invocations_H.irqcontrol_invocation \<Rightarrow> unit kernel_p"
+where
+ "performIRQControl \<equiv> InterruptDecls_H.performIRQControl"
 
 defs decodeIRQControlInvocation_def:
 "decodeIRQControlInvocation label args srcSlot extraCaps \<equiv>
-    (case (invocationType label,args,extraCaps) of
-          (IRQIssueIRQHandler,irqW#index#depth#_,cnode#_) \<Rightarrow>   (doE
-            rangeCheck irqW
-                (fromEnum minIRQ) (fromEnum maxIRQ);
+    (case (invocationType label, args, extraCaps) of
+          (IRQIssueIRQHandler, irqW#index#depth#_, cnode#_) \<Rightarrow>   (doE
+            rangeCheck irqW (fromEnum minIRQ) (fromEnum maxIRQ);
             irq \<leftarrow> returnOk ( toEnum (fromIntegral irqW) ::irq);
             irqActive \<leftarrow> withoutFailure $ isIRQActive irq;
             whenE irqActive $ throw RevokeFirst;
@@ -68,20 +37,17 @@ defs decodeIRQControlInvocation_def:
             returnOk $ IssueIRQHandler irq destSlot srcSlot
           odE)
         | (IRQIssueIRQHandler,_,_) \<Rightarrow>   throw TruncatedMessage
-        | (IRQInterruptControl,_,_) \<Rightarrow>   liftME InterruptControl $
-            ArchInterrupt_H.decodeInterruptControl args extraCaps
-        | _ \<Rightarrow>   throw IllegalOperation
+        | _ \<Rightarrow>   liftME ArchInvokeIRQControl $ ArchInterruptDecls_H.decodeIRQControl label args srcSlot extraCaps
         )"
 
-defs invokeIRQControl_def:
-"invokeIRQControl x0\<equiv> (case x0 of
+defs performIRQControl_def:
+"performIRQControl x0\<equiv> (case x0 of
     (IssueIRQHandler irq handlerSlot controlSlot) \<Rightarrow>   
   withoutPreemption $ (do
     setIRQState (IRQSignal) irq;
     cteInsert (IRQHandlerCap irq) controlSlot handlerSlot
   od)
-  | (InterruptControl invok) \<Rightarrow>   
-    ArchInterrupt_H.invokeInterruptControl invok
+  | (ArchInvokeIRQControl i) \<Rightarrow>    ArchInterruptDecls_H.performIRQControl i
   )"
 
 defs decodeIRQHandlerInvocation_def:
