spec/design/skel/ARM/ArchInvocationLabels_H.thy
@@ -1,0 +1,24 @@
+(*
+ * Copyright 2014, General Dynamics C4 Systems
+ *
+ * This software may be distributed and modified according to the terms of
+ * the GNU General Public License version 2. Note that NO WARRANTY is provided.
+ * See "LICENSE_GPLv2.txt" for details.
+ *
+ * @TAG(GD_GPL)
+ *)
+
+chapter "Architecture-specific Invocation Labels"
+
+theory ArchInvocationLabels_H
+imports "../../../lib/Enumeration"
+begin
+
+text {*
+  An enumeration of arch-specific system call labels.
+*}
+
+#INCLUDE_HASKELL SEL4/API/InvocationLabels/ARM.lhs ONLY ArchInvocationLabel 
+#INCLUDE_HASKELL SEL4/API/InvocationLabels/ARM.lhs instanceproofs ONLY ArchInvocationLabel
+
+end
