spec/design/skel/ARM/ArchVSpaceDecls_H.thy
@@ -1,0 +1,20 @@
+(*
+ * Copyright 2014, General Dynamics C4 Systems
+ *
+ * This software may be distributed and modified according to the terms of
+ * the GNU General Public License version 2. Note that NO WARRANTY is provided.
+ * See "LICENSE_GPLv2.txt" for details.
+ *
+ * @TAG(GD_GPL)
+ *)
+
+chapter "Retyping Objects"
+
+theory ArchVSpaceDecls_H
+imports ArchRetypeDecls_H "../InvocationLabels_H"
+begin
+
+#INCLUDE_HASKELL_PREPARSE SEL4/Object/Structures.lhs
+#INCLUDE_HASKELL SEL4/Kernel/VSpace/ARM.lhs decls_only ArchInv=ArchRetypeDecls_H ArchLabels=ArchInvocationLabels_H
+
+end
