spec/design/skel/ARM/ArchVSpace_H.thy
@@ -1,0 +1,28 @@
+(*
+ * Copyright 2014, General Dynamics C4 Systems
+ *
+ * This software may be distributed and modified according to the terms of
+ * the GNU General Public License version 2. Note that NO WARRANTY is provided.
+ * See "LICENSE_GPLv2.txt" for details.
+ *
+ * @TAG(GD_GPL)
+ *)
+
+(* 
+  VSpace lookup code.
+*)
+
+theory ArchVSpace_H
+imports
+  "../CNode_H"
+  "../KI_Decls_H"
+  ArchVSpaceDecls_H
+begin
+
+#INCLUDE_HASKELL SEL4/Kernel/VSpace/ARM.lhs bodies_only ArchInv=ArchRetypeDecls_H ArchLabels=ArchInvocationLabels_H NOT checkPDAt checkPTAt checkPDASIDMapMembership checkValidMappingSize
+
+defs checkValidMappingSize_def:
+  "checkValidMappingSize sz \<equiv> stateAssert
+    (\<lambda>s. 2 ^ pageBitsForSize sz <= gsMaxObjectSize s) []"
+
+end
