spec/design/skel/Interrupt_H.thy
@@ -11,14 +11,19 @@
 theory Interrupt_H
 imports
   RetypeDecls_H
-  ArchInterrupt_H
+  "./$L4V_ARCH/ArchInterrupt_H"
   Notification_H
   CNode_H
   KI_Decls_H
+  InterruptDecls_H
 begin
 
+abbreviation (input)
+  performIRQControl :: "Invocations_H.irqcontrol_invocation \<Rightarrow> unit kernel_p"
+where
+ "performIRQControl \<equiv> InterruptDecls_H.performIRQControl"
+
 #INCLUDE_HASKELL_PREPARSE SEL4/Object/Structures.lhs
-#INCLUDE_HASKELL SEL4/Object/Interrupt.lhs Arch=ArchInterrupt_H decls_only NOT deletedIRQHandler
-#INCLUDE_HASKELL SEL4/Object/Interrupt.lhs Arch=ArchInterrupt_H bodies_only
+#INCLUDE_HASKELL SEL4/Object/Interrupt.lhs Arch=ArchInterruptDecls_H bodies_only
 
 end
